correct way to define mreg_eqb, (much) more brief way to define mreg_eqb

backend/LTL_PDG_Toy.v
@@ -3,21 +3,70 @@ Require Import AST Integers Values Events Memory Globalenvs Smallstep.
 Require Import Op Locations . *)
 
 (* Require Import Op Locations Conventions. *)
-Require Import Coqlib Maps.
+Require Import Coqlib Maps Integers BoolEqual.
+Require Import AST Linking.
+Require Import Values Memory Events Globalenvs Smallstep.
+Require Import Op Registers Conventions Tailcall.
 Require Import Machregs LTL.
 
+Locate eqb_mreg.
 
-Definition boolTODO:= false.
+Definition mreg_eqb: mreg->mreg->bool.
+Proof. boolean_equality. Defined.
 
-Locate mreg.
-Check mreg_eq.
-Print mreg_eq.
+Lemma mreg_eqb2eq: forall x y, mreg_eqb x y = true -> x = y.
+Proof. BE.bool_eq_sound. Qed.  
 
-Definition eqb_mreg (reg1 reg2: mreg) :=
-    match reg1, reg2 with
-    | AX, AX => true
-    | _, _ => boolTODO
+(** [i1: reg = ...] :: [i2: ... = op args] :: [...] *)
+Fixpoint mregs_depends_on_mreg (args: list mreg) (reg: mreg):=
+    match args with
+    | nil => false
+    | reg' :: args' => if mreg_eqb reg reg' then true 
+                    else mregs_depends_on_mreg args' reg 
     end.
+
+(* (src register, 0:read/1:write/None mem) *)
+Definition get_dst_and_mem (i: instruction): option mreg * option bool :=
+    match i with
+    | Lop op args res => (res, None)
+    | Lload _ _ 
+    | _ => (None, None)
+    end. 
+
+Definition get_srcs_and_mem (i: instruction): list mreg * option bool :=
+    match i with
+    | Lop op args res => (res, None)
+    | _ => (AX, Some true)
+    end. 
+    
+(* i1 depends on i2, i1 <~D i2 *)
+Definition data_depends_on (i1 i2: instruction):=
+    match get_src_and_mem i1, get_dst_and_mem i2 with 
+    (* memory dependence without alias information 
+        - any two memory access with 1 write are regarded to have dependence *)
+    | (_, Some true), (_, Some wr) => true
+    | (_, Some wr), (_, Some true) => true
+    (** register dependence *)
+    | _, _ => false
+    end.
+
+    Notation "i2 D~> i1":= (data_depends_on i1 i2) (at level 1).
+    Notation "i1 <~D i2":= (data_depends_on i1 i2) (at level 1).
+
+(* Definition data_depends_on (i1 i2: instruction): bool :=
+    match i1, i2 with 
+    | Lop op1 args1 res1, Lop op2 args2 res2  => mregs_depends_on_mreg args1 res2
+        | Lop op1 args1 res1, Lload chunk2 addr2 args2 dst2 => mregs_depends_on_mreg args1 dst2
+        | Lop op1 args1 res1, Lgetstack sl2 ofs2 ty2 dst2 => mregs_depends_on_mreg args1 dst2
+        | Lop op1 args1 res1, Lsetstack src2 sl2 ofs2 ty2 => false
+        | Lop op1 args1 res1, Lstore chunk2 addr2 args2 src =>'
+        | Lop op1 args1 res1, _ => boolTODO
+    | Lload chunk addr args dst, _ => boolTODO
+    | _, _ => boolTODO
+    end. *)
+
+
+
 
 Fixpoint mregs_independ_mreg (args: list mreg) (reg: mreg):=
     match args with
@@ -26,14 +75,12 @@ Fixpoint mregs_independ_mreg (args: list mreg) (reg: mreg):=
                     else mregs_independ_mreg args' reg 
     end.
 
-Definition independ_of (i1 i2: instruction) :=
-    match i1 with 
-    | Lop op1 args1 res1  => 
-        match i2 with
-        | Lop op2 args2 res2 => mregs_independ_mreg  args1 res2
-        | _ => boolTODO
-        end
-    | _ => boolTODO
+Definition independ_of (i1 i2: instruction): bool :=
+    match i1, i2 with 
+    | Lop op1 args1 res1, Lop op2 args2 res2  => mregs_independ_mreg  args1 res2
+    | Lop op1 args1 res1, _ => boolTODO
+    | Lload chunk1 addr1 args1 dst1, _ => boolTODO
+    | _, _ => boolTODO
     end.
 
 Require Import AST.
@@ -41,13 +88,194 @@ Require Import Errors.
 Open Scope error_monad_scope.
 
 
-
-(* Definition transf_program (p: LTL.program) : res LTL.program :=
-    transform_partial_program transf_fundef p. *)
-
+(** a meaningless but correct transform function: 
+    exchange the first 2 insttructions of a if possible **)
 
 
+Definition swap_fst_snd_inst (bb: bblock): bblock:=
+    match bb with
+    | i1 :: i2 :: l => if depends_on i2 i1 then bb 
+                        else i2 :: i1 :: l
+    | _ => bb
+    end.
 
+Print mkfunction. 
+Print PTree.elements. 
+Print PTree.map1.
+
+
+Inductive match_stackframes: LTL.stackframe -> LTL.stackframe -> Prop :=
+| match_stackframes_intro:
+    forall f sp ls bb,
+    match_stackframes
+        (Stackframe f sp ls bb)
+        (Stackframe f sp ls bb).
+
+
+Inductive match_local: LTL.state -> LTL.state -> Prop :=
+| match_local_block:
+    forall s f f' sp bb ls m ts tls tm
+    (STK: True)
+    (FUN: True) (STKPTR: True)
+    (LS: ls = tls)
+    (MEM: m = tm),
+    match_local (Block s f sp bb ls m)
+                (Block ts f' sp bb tls tm)
+.
+
+Section TWO_STEP_CORRECTNESS.
+
+Variable prog: LTL.program.
+Variable tprog: LTL.program.
+
+(* Hypothesis TRANSF: match_prog prog tprog. *)
+
+Let ge := Genv.globalenv prog.
+Let tge := Genv.globalenv tprog.
+
+Lemma independ_two_step_match:
+  forall stk1 f sp bb ls m1
+    s1 s3 s1' s3' i1 i2 t t'
+    (* (TRANSF: transf_function f = OK f') *)
+    (INDEP: depends_on i2 i1 = false)
+    (S1: s1 = Block stk1 f sp (i1::i2::bb) ls m1)
+    (STEP13: starN step ge 2 s1 t s3)
+    (S1': s1' = Block stk1 f sp (i2::i1::bb) ls m1)
+    (STEP13': starN step ge 2 s1' t' s3'),
+        t = t' /\ match_local s3 s3'.
+Proof.
+    intros.
+    
+    inv STEP13. rename s' into s2. inv H1. inv H3. rename t0 into t2.
+    inv STEP13'. rename s' into s2'. inv H3. inv H5. rename t0 into t1'. rename t4 into t2'.
+
+    inv H0.
+    - inv H1.
+        + inv H2. inv H4. split; auto. apply match_local_block; auto. 
+            Print Locations.Locmap.set.
+Admitted.
+
+End TWO_STEP_CORRECTNESS.
+
+
+
+Definition transf_code (co: LTL.code): LTL.code :=
+    PTree.map1 swap_fst_snd_inst co.
+
+(* Definition transf_code (co: LTL.code) (entry: node): res LTL.code :=
+    match co!entry with
+    | Some bb => OK (PTree.set entry (swap_fst_inst bb) co)
+    | None => OK co
+    end. *)
+
+Definition transf_function (f: LTL.function) : LTL.function :=
+    let code' := transf_code(fn_code f) in
+    (mkfunction (fn_sig f) (fn_stacksize f) (code') (fn_entrypoint f))
+    . 
+
+Definition transf_fundef (f: LTL.fundef) : res LTL.fundef :=
+    AST.transf_partial_fundef transf_function f.
+
+Definition transf_program (p: LTL.program) : res LTL.program :=
+    transform_partial_program transf_fundef p.
+
+
+
+
+(** Correctness Proof **)
+Print match_program.
+Definition match_prog (p: LTL.program) (tp: LTL.program) :=
+  match_program (fun ctx f tf => transf_fundef f = OK tf) eq p tp.
+
+Lemma transf_program_match:
+  forall p tp, transf_program p = OK tp -> match_prog p tp.
+Proof.
+  intros. eapply match_transform_partial_program; eauto.
+Qed.
+
+Section TOY_CORRECTNESS.
+
+Variable prog: LTL.program.
+Variable tprog: LTL.program.
+
+Hypothesis TRANSF: match_prog prog tprog.
+
+Let ge := Genv.globalenv prog.
+Let tge := Genv.globalenv tprog.
+
+
+Definition locmap_lessdef (ls1 ls2: locset) : Prop :=
+  forall l, Val.lessdef (ls1 l) (ls2 l).
+
+
+
+
+Lemma independ_two_step_match:
+  forall stk1 f f' sp bb ls m 
+    s1 s3 s1' i1 i2 t
+    (TRANSF: transf_function f = OK f')
+    (S1: s1 = Block stk1 f sp (i1::i2::bb) ls m)
+    (STEP13: starN step ge 2 s1 t s3)
+    (MATCH: match_states s1 s1'),
+      exists s3', starN step ge 2 s1' t s3' /\ match_states s3 s3'.
+Proof.
+    intros. inv STEP13. rename s' into s2.
+    inv H1. inv H3.
+
+    inv H0.
+    - 
+Admitted.
+
+
+
+Definition measure (S: LTL.state) := O. 
+
+
+Lemma transf_star2_correct:
+    forall s1 t s2, starN step ge 2 s1 t s2 ->
+        forall s1' (MS: match_states s1 s1'),
+            (exists s2', plus LTL.step tge s1' t s2' /\ match_states s2 s2')
+            \/ (measure s2 < measure s1 /\ t = E0 /\ match_states s2 s1')%nat.
+Proof.
+
+
+Theorem transf_step_correct:
+  forall s1 t s2, LTL.step ge s1 t s2 ->
+  forall s1' (MS: match_states s1 s1'),
+  (exists s2', plus LTL.step tge s1' t s2' /\ match_states s2 s2')
+  \/ (measure s2 < measure s1 /\ t = E0 /\ match_states s2 s1')%nat.
+Proof.
+    induction 1; intros; inv MS. 
+
+Qed.
+
+
+Lemma transf_initial_states:
+forall st1, LTL.initial_state prog st1 ->
+exists st2, LTL.initial_state tprog st2 /\ match_states st1 st2.
+Proof. 
+    intros. inversion H.
+    
+
+Admitted.
+
+Lemma transf_final_states:
+  forall st1 st2 r,
+  match_states st1 st2 -> LTL.final_state st1 r -> LTL.final_state st2 r.
+Proof. Admitted.
+
+
+
+
+Theorem toy_transf_correct:
+  forward_simulation (LTL.semantics prog) (LTL.semantics tprog).
+Proof.
+    eapply forward_simulation_star. 
+    admit. 
+    eexact transf_initial_states.
+    eexact transf_final_states.
+    eexact transf_step_correct.  
+Admitted.
 
 
 
